Working on beginning proofs of TPOSR

proof/TPOSR/CtxReduction.v
@@ -1,10 +1,13 @@
+Require Import Lambda.Tactics.
+Require Import Lambda.Utils.
+
 Require Import Lambda.TPOSR.Terms.
 Require Import Lambda.TPOSR.Reduction.
 Require Import Lambda.TPOSR.Conv.
 Require Import Lambda.TPOSR.LiftSubst.
 Require Import Lambda.TPOSR.Env.
 Require Import Lambda.TPOSR.Types.
-Require Import Lambda.TPOSR.Basic.
+Require Import Lambda.TPOSR.Thinning.
 
 Set Implicit Arguments.
 
@@ -17,127 +20,175 @@ Inductive red_in_env : lenv -> lenv -> Prop :=
   | red_env_hd : forall e t u s, e |-- t -> u : Srt_l s -> e |-- u -> u : Srt_l s ->
 	red_in_env (t :: e) (u :: e)
   | red_env_tl :
-      forall e f t, red_in_env e f -> red_in_env (t :: e) (t :: f).
+      forall e f t, red_in_env e f -> 
+      forall s, f |-- t -> t : Srt_l s ->
+      red_in_env (t :: e) (t :: f).
 
 Hint Resolve red_env_hd red_env_tl: coc.
 
-Lemma red_env :
-  (forall e t u T, e |-- t -> u : T -> 
-  forall f, red_in_env e f -> f |-- t -> u : T).
-Proof.
-Admitted.
-(*
-Lemma ind_conv_env :
-  (forall e t T, e |-- t : T -> 
-  forall f, conv_in_env e f -> f |-- t : T) /\
-  (forall e T U s, e |-- T >> U : s -> 
-  forall f, conv_in_env e f -> f |-- T >> U : s) /\
-  (forall e U V T, e |-- U = V : T ->
-  forall f, conv_in_env e f -> f |-- U = V : T).
-Proof.
-apply typ_coerce_jeq_ind with 
-(P := fun e t T => fun H : typ e t T =>
-  forall f, conv_in_env e f -> 
-  typ f t T)
-(P0 := fun e T U s => fun H : e |-- T >> U : s =>
-  forall f, conv_in_env e f -> 
-  f |-- T >> U : s) 
-(P1 := fun e U V T => fun H : e |-- U = V : T =>
-  forall f, conv_in_env e f -> 
-  f |-- U = V : T) ;
- intros ; try (solve [destruct (H f H0) ; clear H]); 
-auto with coc core arith datatypes.
+Lemma red_item :
+   forall n t e,
+   item_llift t e n ->
+   forall f, red_in_env e f ->
+   item_llift t f n \/
+   ((forall g, trunc _ (S n) e g -> trunc _ (S n) f g) /\
+   exists u, item_llift u f n /\ (exists s : sort, f |-- t -> u : s /\ f |-- u -> u : s)).
+simple induction n.
+do 3 intro.
+elim H.
+do 4 intro.
+rewrite H0.
+inversion_clear H1.
+intros.
+inversion_clear H1.
+right.
+split; intros.
+inversion_clear H1; auto with coc core arith datatypes.
 
-inversion H ; auto with coc.
-inversion H ; auto with coc.
+exists (llift 1 u).
+split.
+inversion_clear H.
 
-inversion H0.
-apply type_conv with (lift 1 u) s0 ; auto with coc.
-apply type_var with s0 ; auto with coc .
-apply coerce_conv ; auto with coc.
-change (Srt s0) with (lift 1 (Srt s0)).
-apply jeq_weak with s0 ; auto.
-apply jeq_sym ; auto.
+unfold item_llift.
+exists u; auto with coc core arith datatypes.
 
-apply type_var with s ; auto.
+exists s ; auto with coc core.
+change (Srt_l s) with (llift 1 (Srt_l s)).
+split ; apply thinning_n with l ; auto with coc core ;
+apply wf_cons with u s ; auto.
 
-inversion H1.
-apply type_weak with s0 ; auto.
-apply type_weak with s ; auto.
+left.
+exists x; auto with coc core arith datatypes.
 
-apply type_abs with s1 s2 ; auto with coc.
+do 5 intro.
+elim H0.
+do 4 intro.
+rewrite H1.
+inversion_clear H2.
+intros.
+inversion_clear H2.
+left.
+exists x; auto with coc core arith datatypes.
 
-apply type_app with V ; auto with coc.
+elim H with (llift (S n0) x) l f0; auto with coc core arith datatypes; intros.
+left.
+elim H2; intros.
+exists x0; auto with coc core arith datatypes.
+rewrite simpl_llift.
+pattern (llift (S (S n0)) x0) in |- *.
+rewrite simpl_llift.
+rewrite H6; auto with coc core arith datatypes.
 
-apply type_pair with s1 s2 s3 ; auto with coc.
+right.
+elim H2.
+clear H2.
+simple induction 2; intros.
+clear H7.
+split; intros.
+inversion_clear H7; auto with coc core arith datatypes.
 
-apply type_prod with s1 ; auto with coc.
+destruct H6.
+destruct H6.
+destruct H7.
+unfold item_llift.
+exists (llift 1 x1).
+split ; auto with coc core.
+inversion_clear H6 ; auto with coc core arith.
+exists x3.
+rewrite H8.
+rewrite <- simpl_llift.
+auto with coc core.
+auto with coc.
 
-apply type_sum with s1 s2 ; auto with coc.
+exists x2.
+pattern (llift (S (S n0)) x) ; rewrite simpl_llift.
+change (Srt_l x2) with (llift 1 (Srt_l x2)).
+destruct H7.
+split ; eapply thinning_n ; auto with coc core ;
+apply wf_cons with y s ; auto.
 
-apply type_subset ; auto with coc.
-
-apply type_pi1 with V ; auto with coc.
-
-apply type_pi2 with U ; auto with coc.
-
-apply type_conv with U s ; auto with coc.
-
-inversion H1.
-apply coerce_weak with s0 ; auto with coc.
-apply coerce_weak with s' ; auto with coc.
-
-apply coerce_prod with s ; auto with coc.
-
-apply coerce_sum with s s' ; auto with coc.
-
-apply coerce_trans with B ; auto with coc.
-
-inversion H1.
-apply jeq_weak with s0 ; auto with coc.
-apply jeq_weak with s ; auto with coc.
-
-apply jeq_prod with s1 ; auto with coc.
-
-apply jeq_abs with s1 s2 ; auto with coc.
-
-apply jeq_app with A ; auto with coc.
-
-apply jeq_beta with s1 s2 ; auto with coc.
-
-apply jeq_red with A s ; auto with coc.
-
-apply jeq_exp with B s ; auto with coc.
-
-apply jeq_sum with s1 s2 ; auto with coc.
-
-apply jeq_pair with s1 s2 s3; auto with coc.
-
-apply jeq_pi1 with  B; auto with coc.
-
-apply jeq_pi1_red with s1 s2 s3; auto with coc.
-
-apply jeq_pi2 with A ; auto with coc.
-
-apply jeq_pi2_red with s1 s2 s3 ; auto with coc.
-
-apply jeq_subset ; auto with coc.
-
-apply jeq_trans with N ; auto with coc.
-
-apply jeq_conv with A s ; auto with coc.
+exists x; auto with coc core arith datatypes.
 Qed.
 
-Lemma type_conv_env : forall e t T, e |-- t : T -> 
-  forall f, conv_in_env e f -> f |-- t : T.
-Proof (proj1 ind_conv_env).
+Lemma ind_red_env :
+  (forall e t u T, e |-- t -> u : T -> 
+  forall f, red_in_env e f -> f |-- t -> u : T) /\
+  (forall e, tposr_wf e -> 
+  forall f, red_in_env e f -> tposr_wf f) /\
+  (forall e t u s, e |-- t ~= u : s -> 
+  forall f, red_in_env e f -> f |-- t ~= u : s) /\
+  (forall e t u s, e |-- t >-> u : s -> 
+  forall f, red_in_env e f -> f |-- t >-> u : s).
+Proof.
+  apply ind_tposr_wf_eq_coerce with
+  (P:=fun e t u T => fun H : e |-- t -> u : T => 
+  forall f, red_in_env e f -> f |-- t -> u : T) 
+  (P0:=fun e => fun H : tposr_wf e => 
+  forall f, red_in_env e f -> tposr_wf f) 
+  (P1:=fun e t u s => fun H : e |-- t ~= u : s => 
+  forall f, red_in_env e f -> f |-- t ~= u : s) 
+  (P2:=fun e t u s => fun H : e |-- t >-> u : s => 
+  forall f, red_in_env e f -> f |-- t >-> u : s) ;
+  intros ; 
+auto with coc core arith datatypes.
 
-Lemma coerce_conv_env : forall e T U s, e |-- T >> U : s -> 
-  forall f, conv_in_env e f -> f |-- T >> U : s.
-Proof (proj1 (proj2 ind_conv_env)).
+destruct (red_item i H0) ; destruct_exists.
+apply tposr_var ; auto with coc.
+apply tposr_conv with x x0 ; auto with coc.
+apply tposr_coerce_sym.
+apply tposr_coerce_conv ; eauto with coc.
 
-Lemma jeq_conv_env : forall e U V T, e |-- U = V : T ->
-  forall f, conv_in_env e f -> f |-- U = V : T.
-Proof (proj2 (proj2 ind_conv_env)).
+apply tposr_prod with s1 ; eauto with coc.
 
-*)
+apply tposr_abs with s1 B' s2 ; eauto with coc.
+
+apply tposr_app with A A' s1 s2 ; eauto with coc.
+
+apply tposr_beta with A' s1 B' s2 ; eauto with coc.
+
+apply tposr_conv with A s ; auto with coc.
+
+apply tposr_subset ; eauto with coc.
+
+apply tposr_sum with s1 s2 ; eauto with coc.
+
+apply tposr_pair with s1 s2 s3 ; eauto with coc.
+
+apply tposr_pi1 with s1 s2 s3 ; eauto with coc.
+
+apply tposr_pi1_red with A' s1 B' s2 s3 v' ; eauto with coc.
+
+apply tposr_pi2 with s1 s2 s3 ; eauto with coc.
+
+apply tposr_pi2_red with A' s1 B' s2 s3 u' ; eauto with coc.
+
+inversion H.
+inversion H0.
+subst.
+apply wf_cons with u s0 ; auto.
+apply wf_cons with A s0 ; auto.
+
+apply tposr_eq_trans with X ; auto with coc.
+
+apply tposr_coerce_prod with s ; eauto with coc.
+
+apply tposr_coerce_sum with s s' ; eauto with coc.
+
+apply tposr_coerce_sub_l  ; eauto with coc.
+
+apply tposr_coerce_sub_r  ; eauto with coc.
+
+apply tposr_coerce_trans with B ; auto with coc.
+Qed.
+
+Lemma tposr_red_env : forall e t u T, e |-- t -> u : T -> 
+  forall f, red_in_env e f -> f |-- t -> u : T.
+Proof (proj1 ind_red_env).
+
+Lemma eq_red_env : forall e u v s, e |-- u ~= v : s ->
+  forall f, red_in_env e f -> f |-- u ~= v : s.
+Proof (proj1 (proj2 (proj2 ind_red_env))).
+
+Lemma coerce_red_env : forall e T U s, e |-- T >-> U : s -> 
+  forall f, red_in_env e f -> f |-- T >-> U : s.
+Proof (proj2 (proj2 (proj2 ind_red_env))).
