proof/TPOSR/LeftReflexivity.v
@@ -4,8 +4,6 @@ Require Import Lambda.TPOSR.Conv.
 Require Import Lambda.TPOSR.LiftSubst.
 Require Import Lambda.TPOSR.Env.
 Require Import Lambda.TPOSR.Types.
-Require Import Lambda.TPOSR.Basic.
-Require Import Lambda.TPOSR.CtxReduction.
 
 Set Implicit Arguments.
 
@@ -14,8 +12,82 @@ Implicit Type s : sort.
 Implicit Types A B M N T t u v : lterm.
 Implicit Types e f g : lenv.
 
-Lemma refl_l : forall e u v T, e |-- u -> v : T -> e |-- u -> u : T.
-Admitted.
+Lemma eq_eq_l :   forall e u v s, e |-- u ~= v : s -> e |-- u ~= u : s.
+Proof.
+  intros.
+  apply tposr_eq_trans with v ; auto with coc.
+Qed.
+
+Lemma eq_eq_r :   forall e u v s, e |-- u ~= v : s -> e |-- v ~= v : s.
+Proof.
+  intros.
+  apply tposr_eq_trans with u ; auto with coc.
+Qed.
+
+Lemma coerce_coerce_l :  forall e u v s, e |-- u >-> v : s -> e |-- u >-> u : s.
+Proof.
+  intros.
+  apply tposr_coerce_trans with v ; auto with coc.
+Qed.
+
+Lemma coerce_coerce_r :  forall e u v s, e |-- u >-> v : s -> e |-- v >-> v : s.
+Proof.
+  intros.
+  apply tposr_coerce_trans with u ; auto with coc.
+Qed.
+
+Hint Resolve eq_eq_l eq_eq_r coerce_coerce_l coerce_coerce_r : ecoc.
+
+Lemma ind_left_refl : 
+  (forall e u v T, e |-- u -> v : T -> e |-- u -> u : T) /\
+  (forall e, tposr_wf e -> True) /\
+  (forall e u v s, e |-- u ~= v : s -> True) /\
+(*  e |-- u -> u : s /\ e |-- v -> v : s) /\*)
+  (forall e u v s, e |-- u >-> v : s ->
+  e |-- u -> u : s /\ e |-- v -> v : s).
+Proof.
+  apply ind_tposr_wf_eq_coerce with 
+  (P:=fun e u v T => fun H : e |-- u -> v : T => e |-- u -> u : T) 
+  (P0:=fun e => fun H : tposr_wf e => True) 
+  (P1:=fun e u v s => fun H : e |-- u ~= v : s => True)
+
+  (P2:=fun e u v s => fun H : e |-- u >-> v : s =>
+  e |-- u -> u : s /\ e |-- v -> v : s) ; simpl ; intros ; intuition ; auto with coc.
+
+  apply tposr_prod with s1 ; auto with coc.
+
+  apply tposr_abs with s1 B s2 ; auto with coc.
+
+  apply tposr_app with  A A  s1 s2 ; auto with coc.
+
+  apply tposr_app with A A s1 s2 ; auto with coc.
+  apply tposr_abs with s1 B s2 ; auto with coc.
+  
+  apply tposr_conv with A s ; auto with coc.
+
+  apply tposr_sum with s1 s2 ; auto with coc.
+
+  apply tposr_pair with s1 s2 s3 ; auto with coc.
+
+  apply tposr_pi1 with s1 s2 s3 ; eauto with coc ecoc.
+
+  apply tposr_pi1 with s1 s2 s3 ; eauto with coc ecoc.
+
+  apply tposr_pi2 with s1 s2 s3 ; eauto with coc ecoc.
+
+  apply tposr_pi2 with s1 s2 s3 ; eauto with coc ecoc.
+
+  apply tposr_prod with s ; auto with coc.
+
+  apply tposr_prod with s ; auto with coc.
+
+  apply tposr_sum with s s' ; auto with coc.
+
+  apply tposr_sum with s s' ; auto with coc.
+Qed.
+
+Corollary refl_l : forall e u v T, e |-- u -> v : T -> e |-- u -> u : T.
+Proof (proj1 (ind_left_refl)).
 
 Corollary tposrp_refl_l : forall e A B T, tposrp e A B T -> e |-- A -> A : T.
 Proof.
@@ -23,5 +95,32 @@ Proof.
   apply (refl_l H).
 Qed.
 
+(*Corollary eq_refl_l : forall e u v s, e |-- u ~= v : s -> e |-- u -> u : s.
+Proof.
+  pose (proj1 (proj2 (proj2 (ind_left_refl)))).
+  intros.
+  destruct (a _ _ _ _ H) ; auto.
+Qed. 
 
-Hint Resolve refl_l tposrp_refl_l : coc.
+Corollary eq_refl_r : forall e u v s, e |-- u ~= v : s -> e |-- v -> v : s.
+Proof.
+  pose (proj1 (proj2 (proj2 (ind_left_refl)))).
+  intros.
+  destruct (a _ _ _ _ H) ; auto.
+Qed. *)
+
+Corollary coerce_refl_l : forall e u v s, e |-- u >-> v : s -> e |-- u -> u : s.
+Proof.
+  pose (proj2 (proj2 (proj2 (ind_left_refl)))).
+  intros.
+  destruct (a _ _ _ _ H) ; auto.
+Qed. 
+
+Corollary coerce_refl_r : forall e u v s, e |-- u >-> v : s -> e |-- v -> v : s.
+Proof.
+  pose (proj2 (proj2 (proj2 (ind_left_refl)))).
+  intros.
+  destruct (a _ _ _ _ H) ; auto.
+Qed. 
+
+Hint Resolve refl_l tposrp_refl_l coerce_refl_l coerce_refl_r : coc.
