proof/TPOSR/Substitution.v
@@ -4,9 +4,11 @@ Require Import Lambda.TPOSR.Conv.
 Require Import Lambda.TPOSR.LiftSubst.
 Require Import Lambda.TPOSR.Env.
 Require Import Lambda.TPOSR.Types.
-Require Import Lambda.TPOSR.Basic.
-Require Import Lambda.TPOSR.CtxReduction.
 Require Import Lambda.TPOSR.LeftReflexivity.
+Require Import Lambda.TPOSR.Thinning.
+Require Import Lambda.TPOSR.CtxReduction.
+
+Require Import Coq.Arith.Lt.
 
 Set Implicit Arguments.
 
@@ -14,6 +16,201 @@ Implicit Types i k m n p : nat.
 Implicit Type s : sort.
 Implicit Types A B M N T t u v : lterm.
 Implicit Types e f g : lenv.
+
+Lemma ind_sub_weak : 
+   (forall e t u U, e |-- t -> u : U ->
+   forall g d d' T, g |-- d -> d' : T ->
+   forall f n, sub_in_lenv d T n e f -> trunc _ n f g -> 
+   f |-- (lsubst_rec d t n) -> (lsubst_rec d' u n) : (lsubst_rec d U n)) /\
+   (forall e, tposr_wf e ->
+   forall g d d' T, g |-- d -> d' : T ->
+   forall n f, sub_in_lenv d T n e f -> trunc _ n f g -> 
+   tposr_wf f) /\
+   (forall e t u s, e |-- t ~= u : s ->
+   forall g d d' T, g |-- d -> d' : T ->
+   forall f n, sub_in_lenv d T n e f -> trunc _ n f g -> 
+   f |-- (lsubst_rec d t n) ~= (lsubst_rec d' u n) : s) /\
+   (forall e t u s, e |-- t >-> u : s ->
+   forall g d d' T, g |-- d -> d' : T ->
+   forall f n, sub_in_lenv d T n e f -> trunc _ n f g -> 
+   f |-- (lsubst_rec d t n) >-> (lsubst_rec d' u n) : s).
+Proof.
+apply ind_tposr_wf_eq_coerce with
+   (P:=fun e t u U => fun H : e |-- t -> u : U =>
+   forall g d d' T, g |-- d -> d' : T ->
+   forall f n, sub_in_lenv d T n e f -> trunc _ n f g -> 
+   f |-- (lsubst_rec d t n) -> (lsubst_rec d' u n) : (lsubst_rec d U n))
+   (P0:= fun e => fun H : tposr_wf e =>
+   forall g d d' T, g |-- d -> d' : T ->
+   forall n f, sub_in_lenv d T n e f -> trunc _ n f g -> 
+   tposr_wf f)
+   (P1 := fun e t u s => fun H : e |-- t ~= u : s =>
+   forall g d d' T, g |-- d -> d' : T ->
+   forall f n, sub_in_lenv d T n e f -> trunc _ n f g -> 
+   f |-- (lsubst_rec d t n) ~= (lsubst_rec d' u n) : s)
+   (P2 := fun e t u s => fun H : e |-- t >-> u : s =>
+   forall g d d' T, g |-- d -> d' : T ->
+   forall f n, sub_in_lenv d T n e f -> trunc _ n f g -> 
+   f |-- (lsubst_rec d t n) >-> (lsubst_rec d' u n) : s);
+   simpl in |- *;
+   intros; auto with coc core arith datatypes.
+
+elim (lt_eq_lt_dec n0 n); [ intro Hlt_eq | intro Hlt ].
+elim i.
+elim Hlt_eq; clear Hlt_eq.
+case n; [ intro Hlt | intros n1 Hlt ]; intros.
+inversion_clear Hlt.
+
+simpl in |- *.
+rewrite H3.
+rewrite simpl_lsubst; auto with coc core arith datatypes.
+apply tposr_var; auto with coc core arith datatypes.
+apply (H _ _ _ _ H0 _ _ H1) ; auto.
+exists x; auto with coc core arith datatypes.
+apply nth_sub_sup with d T0 n0 e; auto with coc core arith datatypes.
+
+intro Heq; intros.
+rewrite H3.
+elim Heq.
+rewrite simpl_lsubst; auto with coc core arith datatypes.
+replace x with T0.
+apply thinning_n with g; auto with coc core arith datatypes.
+subst.
+apply (H _ _ _ _ H0 _ _ H1) ; auto.
+
+apply fun_item with e n; auto with coc core arith datatypes.
+apply nth_sub_eq with d f; auto with coc core arith datatypes.
+elim Heq; auto with coc core arith datatypes.
+
+apply tposr_var; auto with coc core arith datatypes.
+apply (H _ _ _ _ H0 _ _ H1) ; auto.
+apply nth_sub_inf with T0 e; auto with coc core arith datatypes.
+
+apply tposr_set ; eauto with coc.
+
+apply tposr_prop ; eauto with coc.
+
+apply tposr_prod with s1 ; eauto with coc ecoc core arith datatypes.
+
+apply tposr_abs with s1 (lsubst_rec d' B' (S n)) s2 ; eauto with coc core arith datatypes.
+
+rewrite distr_lsubst ; auto with coc.
+apply tposr_app with (lsubst_rec d A n) (lsubst_rec d' A' n) s1 s2; eauto with coc core arith datatypes.
+assert(sub_in_lenv d T (S n) (A :: e) (lsubst_rec d A n :: f)).
+apply sub_S ; auto with coc.
+assert(trunc lterm (S n) (lsubst_rec d A n :: f) g).
+apply trunc_S ; auto with coc.
+pose (H0 _ _ _ _ H3 _ _ H6 H7) ; auto with coc.
+
+rewrite distr_lsubst ; auto with coc.
+rewrite distr_lsubst ; auto with coc.
+apply tposr_beta with (lsubst_rec d' A' n) s1  (lsubst_rec d' B' (S n)) s2; eauto with coc core arith datatypes.
+
+apply tposr_conv with (lsubst_rec d A n) s; eauto with coc.
+
+apply tposr_subset ; eauto with coc.
+
+apply tposr_sum with s1 s2; eauto with coc core arith datatypes.
+
+apply tposr_pair with s1 s2 s3 ; eauto with coc.
+rewrite <- distr_lsubst ; eauto with coc.
+
+pose (H _ _ _ _ H2 _ _ H3 H4).
+apply tposr_pi1 with s1 s2 s3 ; eauto with coc.
+assert(sub_in_lenv d T (S n) (A :: e) (lsubst_rec d A n :: f)).
+apply sub_S ; auto with coc.
+assert(trunc lterm (S n) (lsubst_rec d A n :: f) g).
+apply trunc_S ; auto with coc.
+pose (H0 _ _ _ _ H4 _ _ H7 H8) ; auto with coc.
+
+pose (H2 _ _ _ _ (refl_l H4) _ _ H5 H6).
+apply tposr_pi1_red with (lsubst_rec d' A' n) s1 (lsubst_rec d' B' (S n))  s2 s3 (lsubst_rec d' v' n); eauto with coc.
+
+rewrite distr_lsubst.
+simpl.
+pose (H _ _ _ _ H2 _ _ H3 H4).
+apply tposr_pi2 with s1 s2 s3 ; eauto with coc.
+(*assert(sub_in_lenv d T (S n) (A :: e) (lsubst_rec d A n :: f)).
+apply sub_S ; auto with coc.
+assert(trunc lterm (S n) (lsubst_rec d A n :: f) g).
+apply trunc_S ; auto with coc.
+destruct (H0 _ _ _ _ H2 _ _ H7 H8) ; auto with coc.
+*)
+rewrite distr_lsubst.
+simpl.
+
+pose (H2 _ _ _ _ (refl_l H4) _ _ H5 H6).
+apply tposr_pi2_red with (lsubst_rec d' A' n) s1 (lsubst_rec d' B' (S n))  s2 s3 (lsubst_rec d' u' n); eauto with coc.
+(*assert(sub_in_lenv d T (S n) (A'' :: e) (lsubst_rec d A'' n :: f)).
+apply sub_S ; auto with coc.
+assert(trunc lterm (S n) (lsubst_rec d A'' n :: f) g).
+apply trunc_S ; auto with coc.
+destruct (H3 _ _ _ _ (refl_l H4) _ _ H9 H10) ; auto with coc.*)
+
+inversion H0.
+inversion H1 ; subst.
+apply (wf_tposr t).
+inversion H2.
+apply wf_cons with (lsubst_rec d' A' n0) s ; apply (H _ _ _ _ H0 _ _ H7 H8).
+
+apply tposr_eq_tposr ; eauto with coc.
+apply tposr_eq_tposr ; eauto with coc.
+
+apply H1 ; eauto with coc.
+
+eauto with coc.
+
+
+eauto with coc.
+apply tposr_eq_trans with (lsubst_rec d X n).
+apply tposr_eq_sym.
+apply tposr_eq_tposr ; eauto with coc.
+apply tposr_eq_tposr ; eauto with coc.
+
+destruct (H _ _ _ _ H0 _ _ H1 H2).
+split ; auto with coc.
+
+
+destruct (H _ _ _ _ H1 _ _ H2 H3).
+destruct (H0 _ _ _ _ H1 _ _ H2 H3).
+destruct (H0 _ _ _ _ (refl_l H1) _ _ H2 H3).
+destruct (H _ _ _ _ (refl_l H1) _ _ H2 H3).
+split.
+apply tposr_eq_trans with (lsubst_rec d' X n) ; eauto with coc.
+eauto with coc ecoc.
+eauto with coc ecoc.
+
+destruct (H1 _ _ _ _ H2 _ _ H3 H4).
+split ; apply tposr_coerce_conv ; auto with coc.
+eauto with coc.
+pose (coerce_refl
+eauto with coc.
+
+ ; eauto with coc ecoc.
+destruct (H0 _ _ _ _ H1 _ _ H2 H3).
+destruct (H0 _ _ _ _ (refl_l H1) _ _ H2 H3).
+destruct (H _ _ _ _ (refl_l H1) _ _ H2 H3).
+
+
+
+
+assert (tposr_wf (llift_rec 1 A' n :: f)) by (apply wf_cons with (llift_rec 1 A' n) s ; eauto with coc).
+assert (tposr_wf (llift_rec 1 A0 n :: f)) by (apply wf_cons with (llift_rec 1 A0 n) s ; eauto with coc).
+apply tposr_coerce_prod with s ; auto with coc.
+
+assert (tposr_wf (llift_rec 1 A' n :: f)) by (apply wf_cons with (llift_rec 1 A' n) s ; eauto with coc).
+assert (tposr_wf (llift_rec 1 A0 n :: f)) by (apply wf_cons with (llift_rec 1 A0 n) s ; eauto with coc).
+apply tposr_coerce_sum with s s' ; auto with coc.
+
+assert (tposr_wf (llift_rec 1 U n :: f)) by (apply wf_cons with (llift_rec 1 U n) set ; eauto with coc).
+apply tposr_coerce_sub_l ; auto with coc.
+
+assert (tposr_wf (llift_rec 1 U' n :: f)) by (apply wf_cons with (llift_rec 1 U' n) set ; eauto with coc).
+apply tposr_coerce_sub_r ; auto with coc.
+
+apply tposr_coerce_trans with (llift_rec 1 B n) ; auto with coc.
+Qed.
+
 
 Theorem tposr_sub : forall g d d' t, g |-- d -> d' : t ->
    forall e u v U, e |-- u -> v : U ->
@@ -81,171 +278,6 @@ Proof.
   unfold lsubst ; eapply tposr_coerce_sub ; auto with coc.
   apply H0.
   apply H.
-Qed.
-
-(*Lemma ind_sub_weak : forall g (d : term) t, g |-- d : t ->
-   (forall e u (U : term), e |-- u : U ->
-   forall f n, sub_in_env d t n e f -> trunc _ n f g -> 
-   f |-- (subst_rec d u n) : (subst_rec d U n)) /\
-   (forall e T U s, e |-- T >> U : s ->
-   forall f n, sub_in_env d t n e f -> trunc _ n f g -> 
-   f |-- (subst_rec d T n) >> (subst_rec d U n) : s) /\
-   (forall e U V T, e |-- U = V : T ->
-   forall f n, sub_in_env d t n e f -> trunc _ n f g -> 
-   f |-- (subst_rec d U n) = (subst_rec d V n) : (subst_rec d T n)).
-Proof.
-intros g d t H.
-apply typ_coerce_jeq_ind with
-   (P:=fun e u (U : term) => fun H : e |-- u : U =>
-   forall f n, sub_in_env d t n e f -> trunc _ n f g -> 
-   f |-- (subst_rec d u n) : (subst_rec d U n)) 
-   (P1:=fun e U V T => fun H : e |-- U = V : T =>
-   forall f n, sub_in_env d t n e f -> trunc _ n f g -> 
-   f |-- (subst_rec d U n) = (subst_rec d V n) : (subst_rec d T n))
-   (P0:=fun e T U s => fun H : e |-- T >> U : s =>
-   forall f n, sub_in_env d t n e f -> trunc _ n f g -> 
-   f |-- (subst_rec d T n) >> (subst_rec d U n) : s) ;
- simpl in |- *;
- intros; auto with coc core arith datatypes.
-
-inversion H0.
-
-inversion H0.
-
-elim (lt_eq_lt_dec n 0); [ intro Hlt_eq | intro Hlt ].
-elim Hlt_eq; clear Hlt_eq.
-intros.
-assert(False) ; try omega ; contradiction.
-intros.
-rewrite b ; simpl.
-rewrite simpl_subst ; auto with arith.
-rewrite lift0.
-rewrite lift0.
-rewrite b in H2.
-rewrite b in H1.
-inversion H1.
-inversion H2.
-rewrite <- H3 ; assumption.
-
-inversion H1.
-rewrite <- H3 in Hlt.
-assert(False) ; try omega ; contradiction.
-rewrite commut_lift_subst.
-apply type_var with s.
-apply H0 ; auto.
-rewrite <- H4 in H2.
-rewrite <- H5 in H2.
-inversion H2 ; auto.
-
-inversion H2.
-rewrite simpl_subst ; auto with arith.
-rewrite lift0.
-rewrite simpl_subst ; auto with arith.
-rewrite lift0.
-rewrite <- H5 ; assumption.
-
-rewrite commut_lift_subst.
-rewrite commut_lift_subst.
-rewrite <- H5 in H3.
-rewrite <- H6 in H3.
-inversion H3.
-apply type_weak with s ; auto.
-
-apply type_abs with s1 s2 ; auto with coc.
-
-rewrite distr_subst.
-apply type_app with (subst_rec d V n) ; auto with coc.
-
-apply type_pair with s1 s2 s3 ; auto with coc.
-rewrite <- distr_subst ; auto with coc.
-
-apply type_prod with s1 ; auto with coc.
-
-apply type_sum with s1 s2 ; auto with coc.
-
-apply type_subset ; auto with coc.
-
-apply type_pi1 with (subst_rec d V (S n)) ; auto with coc.
-
-rewrite distr_subst.
-simpl.
-apply type_pi2 with (subst_rec d U n) ; auto with coc.
-
-apply type_conv with (subst_rec d U n) s ; auto with coc.
-
-inversion H2.
-rewrite simpl_subst ; auto with arith.
-rewrite simpl_subst ; auto with arith.
-rewrite lift0 ; rewrite lift0.
-rewrite <- H5 ; auto.
-rewrite <- H5 in H3.
-rewrite <- H6 in H3.
-inversion H3.
-
-rewrite commut_lift_subst.
-rewrite commut_lift_subst.
-apply coerce_weak with s' ; auto with coc.
-
-apply coerce_prod with s ; auto with coc.
-
-apply coerce_sum with s s' ; auto with coc.
-
-apply coerce_trans with (subst_rec d B n) ; auto with coc.
-
-inversion H2.
-do 3 (rewrite simpl_subst ; auto with arith).
-do 3 rewrite lift0.
-rewrite <- H5 ; auto.
-rewrite <- H5 in H3.
-rewrite <- H6 in H3.
-inversion H3.
-
-do 3 (rewrite commut_lift_subst).
-apply jeq_weak with s ; auto with coc.
-
-apply jeq_prod with s1 ; auto with coc.
-
-apply jeq_abs with s1 s2 ; auto with coc.
-
-rewrite distr_subst.
-apply jeq_app with (subst_rec d A n) ; auto with coc.
-
-rewrite distr_subst.
-rewrite distr_subst.
-apply jeq_beta with s1 s2 ; auto with coc.
-
-apply jeq_red with (subst_rec d A n) s ; auto with coc.
-
-apply jeq_exp with (subst_rec d B n) s ; auto with coc.
-
-apply jeq_sum with s1 s2 ; auto with coc.
-
-apply jeq_pair with s1 s2 s3 ; auto with coc.
-simpl.
-rewrite <- distr_subst.
-apply H3 ; auto with coc.
-
-apply jeq_pi1 with (subst_rec d B (S n)) ; auto with coc.
-
-apply jeq_pi1_red with s1 s2 s3 ; auto with coc.
-rewrite <- distr_subst.
-apply H3 ; auto with coc.
-
-rewrite distr_subst.
-simpl.
-apply jeq_pi2 with (subst_rec d A n) ; auto with coc.
-
-rewrite distr_subst.
-apply jeq_pi2_red with s1 s2 s3; auto with coc.
-rewrite <- distr_subst.
-apply H3 ; auto with coc.
-
-
-apply jeq_subset ; auto with coc.
-
-apply jeq_trans with (subst_rec d N n) ; auto with coc.
-
-apply jeq_conv with (subst_rec d A n) s ; auto with coc.
 Qed.
 
 Lemma typ_sub_weak : forall g (d : term) t, g |-- d : t ->
