proof/TPOSR/Thinning.v
@@ -4,7 +4,7 @@ Require Import Lambda.TPOSR.LiftSubst.
 Require Import Lambda.TPOSR.Env.
 Require Import Lambda.TPOSR.Conv.
 Require Import Lambda.TPOSR.Types.
-Require Import Lambda.TPOSR.Basic.
+Require Import Lambda.TPOSR.LeftReflexivity.
 
 Set Implicit Arguments.
 
@@ -13,20 +13,32 @@ Implicit Type s : sort.
 Implicit Types A B M N T t u v : lterm.
 Implicit Types e f g : lenv.
 
-Lemma weak_weak : forall A,
+Lemma ind_thinning : forall A,
   (forall e u v T, e |-- u -> v : T ->
-   forall n f, ins_in_lenv A n e f -> tposr_wf f -> 
+   forall n f, ins_in_lenv A n e f -> tposr_wf f ->
    f |-- (llift_rec 1 u n) -> (llift_rec 1 v n) : (llift_rec 1 T n)) /\
+  (forall e, tposr_wf e -> True) /\
   (forall e u v s, e |-- u ~= v : s ->
-   forall n f, ins_in_lenv A n e f -> tposr_wf f -> 
-   f |-- (llift_rec 1 u n) ~= (llift_rec 1 v n) : s).
-Admitted.
-(*Proof.
+   forall n f, ins_in_lenv A n e f -> tposr_wf f ->
+   f |-- (llift_rec 1 u n) ~= (llift_rec 1 v n) : s) /\
+  (forall e u v s, e |-- u >-> v : s ->
+   forall n f, ins_in_lenv A n e f -> tposr_wf f ->
+   f |-- (llift_rec 1 u n) >-> (llift_rec 1 v n) : s).
+Proof.
 intros A.
-induction 1 using ind_tposr with 
+apply ind_tposr_wf_eq_coerce with 
  (P := fun e u v T => fun IH : e |-- u -> v : T =>
    forall n f,
-   ins_in_lenv A n e f -> tposr_wf f -> f |-- (llift_rec 1 u n) -> (llift_rec 1 v n) : (llift_rec 1 T n)) ;
+   ins_in_lenv A n e f -> tposr_wf f ->
+   f |-- (llift_rec 1 u n) -> (llift_rec 1 v n) : (llift_rec 1 T n))
+  (P0 := fun e => fun H : tposr_wf e => 
+   True)
+  (P1 := fun e u v s => fun H : e |-- u ~= v : s =>
+   forall n f, ins_in_lenv A n e f -> tposr_wf f ->
+   f |-- (llift_rec 1 u n) ~= (llift_rec 1 v n) : s)
+  (P2 := fun e u v s => fun H : e |-- u >-> v : s =>
+   forall n f, ins_in_lenv A n e f -> tposr_wf f ->
+   f |-- (llift_rec 1 u n) >-> (llift_rec 1 v n) : s) ;
    simpl in |- *; 
    try simpl in IHtposr1 ; 
    try simpl in IHtposr0 ; 
@@ -40,7 +52,7 @@ elim (le_gt_dec n0 n); intros; apply tposr_var;
  auto with coc core arith datatypes.
 elim i; intros.
 exists x.
-rewrite H1.
+rewrite H2.
 unfold llift in |- *.
 rewrite simpl_llift_rec; simpl in |- *; auto with coc core arith datatypes.
 
@@ -48,71 +60,100 @@ apply ins_item_ge with A n0 e; auto with coc core arith datatypes.
 
 apply ins_item_lt with A e; auto with coc core arith datatypes.
 
-assert (tposr_wf (llift_rec 1 A0 n :: f)) by apply wf_cons with (llift_rec 1 A' n) s1 ; auto with coc.
+assert (tposr_wf (llift_rec 1 A0 n :: f)) by (apply wf_cons with (llift_rec 1 A' n) s1 ; auto with coc).
 apply tposr_prod with s1 ; auto with coc core arith datatypes.
 
-assert (tposr_wf (llift_rec 1 A0 n :: f)) by apply wf_cons with (llift_rec 1 A' n) s1 ; auto with coc.
+assert (tposr_wf (llift_rec 1 A0 n :: f)) by (apply wf_cons with (llift_rec 1 A' n) s1 ; auto with coc).
 apply tposr_abs with s1 (llift_rec 1 B' (S n)) s2 ; auto with coc core arith datatypes.
 
-assert (tposr_wf (llift_rec 1 A0 n :: f)) by apply wf_cons with (llift_rec 1 A' n) s1 ; auto with coc.
+assert (tposr_wf (llift_rec 1 A0 n :: f)) by (apply wf_cons with (llift_rec 1 A' n) s1 ; auto with coc).
 rewrite distr_llift_lsubst ; auto with coc.
 apply tposr_app with (llift_rec 1 A0 n) (llift_rec 1 A' n) s1 s2; auto with coc core arith datatypes.
 
-
-assert (tposr_wf (llift_rec 1 A0 n :: f)) by apply wf_cons with (llift_rec 1 A' n) s1 ; auto with coc.
+assert (tposr_wf (llift_rec 1 A0 n :: f)) by (apply wf_cons with (llift_rec 1 A' n) s1 ; auto with coc).
 rewrite distr_llift_lsubst ; auto with coc.
 rewrite distr_llift_lsubst ; auto with coc.
 
 apply tposr_beta with (llift_rec 1 A' n) s1 (llift_rec 1 B' (S n)) s2; auto with coc core arith datatypes.
 
-apply tposr_red with (llift_rec 1 A0 n) s; auto with coc.
+apply tposr_conv with (llift_rec 1 A0 n) s; auto with coc.
 
-apply tposr_exp with (llift_rec 1 B n) s; auto with coc.
-
-assert (tposr_wf (llift_rec 1 A0 n :: f)) by apply wf_cons with (llift_rec 1 A' n) set ; auto with coc.
+assert (tposr_wf (llift_rec 1 A0 n :: f)) by (apply wf_cons with (llift_rec 1 A' n) set ; auto with coc).
 apply tposr_subset ; auto with coc.
 
-assert (tposr_wf (llift_rec 1 A0 n :: f)) by apply wf_cons with (llift_rec 1 A' n) s1 ; auto with coc.
+assert (tposr_wf (llift_rec 1 A0 n :: f)) by (apply wf_cons with (llift_rec 1 A' n) s1 ; auto with coc).
 apply tposr_sum with s1 s2; auto with coc core arith datatypes.
 
-assert (tposr_wf (llift_rec 1 A0 n :: f)) by apply wf_cons with (llift_rec 1 A' n) s1 ; auto with coc.
+assert (tposr_wf (llift_rec 1 A0 n :: f)) by (apply wf_cons with (llift_rec 1 A' n) s1 ; auto with coc).
 apply tposr_pair with s1 s2 s3 ; auto with coc.
 rewrite <- distr_llift_lsubst ; auto with coc.
 
-assert (tposr_wf (llift_rec 1 A0 n :: f)) by apply wf_cons with (llift_rec 1 A' n) s1 ; auto with coc.
 apply tposr_pi1 with s1 s2 s3 ; auto with coc.
+apply H0 ; eauto with coc .
+apply wf_cons with (llift_rec 1 A0 n) s1 ; eauto with coc.
 
-assert (tposr_wf (llift_rec 1 A0 n :: f)) by apply wf_cons with (llift_rec 1 A' n) s1 ; auto with coc.
-assert (tposr_wf (llift_rec 1 A'' n :: f)) by apply wf_cons with (llift_rec 1 A' n) s1 ; auto with coc.
+assert (tposr_wf (llift_rec 1 A0 n :: f)) by (apply wf_cons with (llift_rec 1 A0 n) s1 ; eauto with coc).
+assert (tposr_wf (llift_rec 1 A'' n :: f)) by (apply wf_cons with (llift_rec 1 A'' n) s1 ; eauto with coc).
 apply tposr_pi1_red with (llift_rec 1 A' n) s1 (llift_rec 1 B' (S n))  s2 s3 (llift_rec 1 v' n); auto with coc.
 
-assert (tposr_wf (llift_rec 1 A0 n :: f)) by apply wf_cons with (llift_rec 1 A' n) s1 ; auto with coc.
+assert (tposr_wf (llift_rec 1 A0 n :: f)) by (apply wf_cons with (llift_rec 1 A0 n) s1 ; eauto with coc).
 rewrite distr_llift_lsubst.
 simpl.
 apply tposr_pi2 with s1 s2 s3 ; auto with coc.
 
-assert (tposr_wf (llift_rec 1 A0 n :: f)) by apply wf_cons with (llift_rec 1 A' n) s1 ; auto with coc.
+assert (tposr_wf (llift_rec 1 A0 n :: f)) by (apply wf_cons with (llift_rec 1 A0 n) s1 ; eauto with coc).
+assert (tposr_wf (llift_rec 1 A'' n :: f)) by (apply wf_cons with (llift_rec 1 A'' n) s1 ; eauto with coc).
 rewrite distr_llift_lsubst.
 simpl.
 apply tposr_pi2_red with (llift_rec 1 A' n) s1 (llift_rec 1 B' (S n))  s2 s3 (llift_rec 1 u' n); auto with coc.
+
+apply tposr_eq_trans with (llift_rec 1 X n) ; auto with coc.
+
+assert (tposr_wf (llift_rec 1 A' n :: f)) by (apply wf_cons with (llift_rec 1 A' n) s ; eauto with coc).
+assert (tposr_wf (llift_rec 1 A0 n :: f)) by (apply wf_cons with (llift_rec 1 A0 n) s ; eauto with coc).
+apply tposr_coerce_prod with s ; auto with coc.
+
+assert (tposr_wf (llift_rec 1 A' n :: f)) by (apply wf_cons with (llift_rec 1 A' n) s ; eauto with coc).
+assert (tposr_wf (llift_rec 1 A0 n :: f)) by (apply wf_cons with (llift_rec 1 A0 n) s ; eauto with coc).
+apply tposr_coerce_sum with s s' ; auto with coc.
+
+assert (tposr_wf (llift_rec 1 U n :: f)) by (apply wf_cons with (llift_rec 1 U n) set ; eauto with coc).
+apply tposr_coerce_sub_l ; auto with coc.
+
+assert (tposr_wf (llift_rec 1 U' n :: f)) by (apply wf_cons with (llift_rec 1 U' n) set ; eauto with coc).
+apply tposr_coerce_sub_r ; auto with coc.
+
+apply tposr_coerce_trans with (llift_rec 1 B n) ; auto with coc.
 Qed.
-*)
-  Theorem thinning :
+
+Corollary thinning :
    forall e t t' T,
-   e |-- t -> t' : T -> forall A, tposr_wf (A :: e) -> (A :: e) |-- (llift 1 t) -> llift 1 t' : (llift 1 T).
+   e |-- t -> t' : T -> forall A, tposr_wf (A :: e) -> (A :: e) |-- llift 1 t -> llift 1 t' : (llift 1 T).
 Proof.
 unfold llift in |- *.
 intros.
-inversion_clear H0.
-apply (proj1 (weak_weak A)) with e ; auto with coc.
-apply wf_cons with A' s; auto with coc core arith datatypes.
+apply (proj1 (ind_thinning A)) with e ; auto with coc.
 Qed.
 
-Lemma thinning_coerce :
+Corollary thinning_eq :
+   forall e t t' s,
+   e |-- t ~= t' : s -> 
+   forall A, tposr_wf (A :: e) -> (A :: e) |-- (llift 1 t) ~= llift 1 t' : s.
+Proof.
+unfold llift in |- *.
+intros.
+apply (proj1 (proj2 (proj2 (ind_thinning A)))) with e ; auto with coc.
+Qed.
+
+Corollary thinning_coerce :
    forall e t t' s,
    e |-- t >-> t' : s -> 
    forall A, tposr_wf (A :: e) -> (A :: e) |-- (llift 1 t) >-> llift 1 t' : s.
-Admitted.
+Proof.
+unfold llift in |- *.
+intros.
+apply (proj2 (proj2 (proj2 (ind_thinning A)))) with e ; auto with coc.
+Qed.
 
 Lemma thinning_n :
    forall n e f,
@@ -141,6 +182,61 @@ apply H with f; auto with coc core arith datatypes.
 apply wf_tposr with x A' (Srt_l s); auto with coc core arith datatypes.
 
 apply wf_cons with A' s; auto with coc core arith datatypes.
+Qed.
+
+
+Lemma thinning_n_eq :
+   forall n e f,
+   trunc _ n e f ->
+   forall t t' s, f |-- t ~= t' : s -> tposr_wf e -> e |-- (llift n t) ~= (llift n t') : s.
+Proof.
+simple induction n.
+intros.
+do 2 rewrite llift0.
+replace e with f; auto with coc core arith datatypes.
+inversion_clear H; auto with coc core arith datatypes.
+
+do 8 intro.
+inversion_clear H0.
+intro.
+rewrite simpl_llift; auto with coc core arith datatypes.
+
+pattern (llift (S n0) t') in |- *.
+rewrite simpl_llift; auto with coc core arith datatypes.
+intros.
+inversion_clear H2.
+apply thinning_eq; auto with coc core arith datatypes.
+apply H with f; auto with coc core arith datatypes.
+apply wf_tposr with x A' (Srt_l s0); auto with coc core arith datatypes.
+
+apply wf_cons with A' s0; auto with coc core arith datatypes.
+Qed.
+
+Lemma thinning_n_coerce :
+   forall n e f,
+   trunc _ n e f ->
+   forall t t' s, f |-- t >-> t' : s -> tposr_wf e -> e |-- (llift n t) >-> (llift n t') : s.
+Proof.
+simple induction n.
+intros.
+do 2 rewrite llift0.
+replace e with f; auto with coc core arith datatypes.
+inversion_clear H; auto with coc core arith datatypes.
+
+do 8 intro.
+inversion_clear H0.
+intro.
+rewrite simpl_llift; auto with coc core arith datatypes.
+
+pattern (llift (S n0) t') in |- *.
+rewrite simpl_llift; auto with coc core arith datatypes.
+intros.
+inversion_clear H2.
+apply thinning_coerce; auto with coc core arith datatypes.
+apply H with f; auto with coc core arith datatypes.
+apply wf_tposr with x A' (Srt_l s0); auto with coc core arith datatypes.
+
+apply wf_cons with A' s0; auto with coc core arith datatypes.
 Qed.
 
 Lemma wf_sort_lift :
@@ -182,4 +278,4 @@ inversion_clear H3.
 apply (wf_tposr H5); auto with coc core arith datatypes.
 Qed.
 
-Hint Resolve thinning thinning_n : coc.
+Hint Resolve thinning thinning_eq thinning_coerce thinning_n : coc.
